src/HOL/Word/Bits.thy
@@ -5,15 +5,11 @@
 section \<open>Syntactic type classes for bit operations\<close>
 
 theory Bits
-  imports Main
+  imports Main "HOL-Library.Bit_Operations"
 begin
 
 class bit_operations =
-  fixes bitNOT :: "'a \<Rightarrow> 'a"  ("NOT")
-    and bitAND :: "'a \<Rightarrow> 'a \<Rightarrow> 'a"  (infixr "AND" 64)
-    and bitOR :: "'a \<Rightarrow> 'a \<Rightarrow> 'a"  (infixr "OR"  59)
-    and bitXOR :: "'a \<Rightarrow> 'a \<Rightarrow> 'a"  (infixr "XOR" 59)
-    and shiftl :: "'a \<Rightarrow> nat \<Rightarrow> 'a"  (infixl "<<" 55)
+  fixes shiftl :: "'a \<Rightarrow> nat \<Rightarrow> 'a"  (infixl "<<" 55)
     and shiftr :: "'a \<Rightarrow> nat \<Rightarrow> 'a"  (infixl ">>" 55)
   fixes test_bit :: "'a \<Rightarrow> nat \<Rightarrow> bool"  (infixl "!!" 100)
     and lsb :: "'a \<Rightarrow> bool"
